assignment targets

src/Sound/VCGen/AssignmentTarget' copy.dfy
@@ -1,429 +1,568 @@
-// module AssignmentTarget' {
-//   import opened Defs
-//   import Omni
+module AssignmentTarget'' {
+  import opened Defs
+  import Omni
 
-//   export
-//     provides Defs, Omni, Process, Correct
-//     reveals PairToSet, EqsTo
+  export
+    provides Defs, Omni, Process, Correct
+    reveals PairToSet, EqsTo
   
-//   predicate ShiftedIn(s: set<Idx>, n: nat, i: Idx) {
-//     i + n in s
-//   }
+  predicate ShiftedIn(s: set<Idx>, n: nat, i: Idx) {
+    i + n in s
+  }
   
 
-//   newtype VarsJumps = map<nat, set<Idx>> {
-//     // function Update(n: nat): VarsJumps {
-//     //   map i: Idx | i in Keys :: if i == 0 then n else Pred(this[i])
-//     // }
+  newtype VarsJumps = map<nat, set<Idx>> {
+    // function Update(n: nat): VarsJumps {
+    //   map i: Idx | i in Keys :: if i == 0 then n else Pred(this[i])
+    // }
 
-//     function Upd0(): VarsJumps {
-//       if 0 in Keys then this else map[0 := {}]
-//     }
+    ghost function Prefix(n: nat): iset<Idx> {
+      iset i: Idx | InPrefix(i, n)
+    }
 
-//     function Merge(m1: VarsJumps): VarsJumps {
-//       var s0 := if 0 in Keys then this[0] else {};
-//       var s1 := if 0 in m1.Keys then m1[0] else {};
-//       map i: Idx | i in Keys + m1.Keys :: 
-//         if i in Keys then
-//           if i in m1.Keys then
-//             this[i] + m1[i]
-//           else this[i] + s1
-//         else m1[i] + s0
-//     }
-
-//     function SeqMerge(m: VarsJumps): VarsJumps {
-//       var s0 := if 0 in Keys then this[0] else {};
-//       map i: nat | i in (Keys - {0}) + m.Keys :: 
-//         if i in Keys then
-//           if i in m.Keys then
-//             this[i] + s0 + m[i]
-//           else this[i] + s0
-//         else m[i] 
-          
-//     }
-
-//     function SubstractSet(n: nat, s: set<Idx>): set<Idx> 
-//       ensures forall i: Idx :: i + n in s ==> i in SubstractSet(n, s)
-//     {
-//       set i: Idx {:trigger i + n in s} | i <= Max'(s) - n && i + n in s 
-//     }
-
-//     lemma InSubstractSet(s: set<Idx>, n: nat, i: Idx) 
-//       requires i + n in s 
-//       ensures i in SubstractSet(n, s)
-//     {
-
-//     }
-
-//     function Substract(n: nat): VarsJumps {
-//       map i: nat | 
-//         && i <= Max'(Keys) + 1
-//         && Pred(i) in Keys :: SubstractSet(n, this[Pred(i)]) 
-//     }
-
-//     lemma SubstractLemma(n: nat, i: nat)
-//       requires Pred(i) in Keys
-//       ensures Substract(n)[i] == SubstractSet(n, this[Pred(i)])
-//     {
-
-//     }
-
-//     // predicate InUpto(i:idx, n: nat) 
-//     //   requires n in Keys
-//     // {
+    ghost predicate InPrefix(i: Idx, n: nat) 
+    {
+      exists k: nat :: k <= n && k in Keys && i in this[k]
+    }
       
-//     // }
 
-//     ghost function ToEqs(st: State, posts: Omni.Continuation): Omni.Continuation 
-//     {
-//       seq(|posts|, (k : nat) requires k < |posts| => 
-//         if k !in Keys then iset{} else
-//         iset st' |
-//           && st' in posts[k]
-//           && |st'| == |st|
-//           && forall i: Idx :: i < |st| && !(k in Keys && i in this[k]) ==> st[i] == st'[i]
-//       )
-//     }
-//   }
+    // ghost function Prefix(n: nat): iset<Idx> 
+    // {
+    //   iset i: Idx | InPrefix(i, n)
+    // }
 
-//   function Pred(n: nat): nat {
-//     if n == 0 then 0 else n - 1
-//   }
+    function Merge(m1: VarsJumps): VarsJumps {
+      map i: Idx | i in Keys + m1.Keys :: 
+        if i in Keys then
+          if i in m1.Keys then
+            this[i] + m1[i]
+          else this[i]
+        else m1[i]
+    }
+
+    function Remove0(): VarsJumps {
+      var s0 := if 0 in Keys then this[0] else {};
+      map i: Idx | i in Keys - {0} :: this[i] + s0
+    }
+
+    function SeqMerge(m: VarsJumps): VarsJumps {
+      var s0 := if 0 in Keys then this[0] else {};
+      map i: nat | i in (Keys - {0}) + m.Keys :: 
+        if i in Keys then
+          if i in m.Keys then
+            this[i] + s0 + m[i]
+          else this[i] + s0
+        else m[i] 
+          
+    }
+
+    function SubstractSet(n: nat, s: set<Idx>): set<Idx> 
+      ensures forall i: Idx :: i + n in s ==> i in SubstractSet(n, s)
+    {
+      set i: Idx {:trigger i + n in s} | i <= Max'(s) - n && i + n in s 
+    }
+
+    lemma InSubstractSet(s: set<Idx>, n: nat, i: Idx) 
+      requires i + n in s 
+      ensures i in SubstractSet(n, s)
+    {
+
+    }
+
+    function Get(i: Idx) : set<Idx> {
+      if i in Keys then this[i] else {}
+    }
+
+    predicate SubstractPred(i: Idx) {
+      i + 1 in Keys
+    }
+
+    predicate Trigger(i: Idx) {
+      true
+    }
+
+    opaque function Substract(n: nat): VarsJumps 
+      ensures forall i: Idx :: i + 1 in Keys ==> i in Substract(n).Keys
+      ensures 0 in Keys ==> 0 in Substract(n).Keys
+      ensures 0 in Substract(n).Keys ==> Substract(n)[0] == SubstractSet(n, this.Get(0) + this.Get(1))
+      ensures forall i: Idx :: (i + 1 in Keys && i != 0) ==> Substract(n)[i] == SubstractSet(n, this[i + 1])
+    {
+      var m: VarsJumps := map i: nat | 
+        && i <= Max'(Keys) + 1
+        && Trigger(i)
+        && i + 1 in Keys :: SubstractSet(n, this[i + 1]);
+      // var s0 := SubstractSet(n, if 0 in Keys then this[0] else {});
+      if 0 in m.Keys && 0 in Keys then 
+        m[0 := m[0] + SubstractSet(n, this[0])]
+      else if 0 in Keys then 
+        m[0 := SubstractSet(n, this[0])]
+      else m
+    }
+
+    // lemma SubstractLemma(n: nat, i: Idx)
+    //   ensures i + 1 in Keys ==> i in Substract(n).Keys
+    //   ensures 0 in Substract(n).Keys ==> Substract(n)[0] == SubstractSet(n, this.Get(0) + this.Get(1))
+    //   ensures (i + 1 in Keys && i != 0) ==> Substract(n)[i] == SubstractSet(n, this[i + 1])
+    // {
+
+    // }
+
+
+    // predicate InUpto(i:idx, n: nat) 
+    //   requires n in Keys
+    // {
+      
+    // }
+
+    ghost function ToEqs(st: State, posts: Omni.Continuation): Omni.Continuation 
+    {
+      seq(|posts|, (k : nat) requires k < |posts| => 
+        if k !in Keys then iset{} else
+        iset st' |
+          && st' in posts[k]
+          && |st'| == |st|
+          && forall i: Idx :: i < |st| && !(i in Prefix(k)) ==> st[i] == st'[i]
+      )
+    }
+
+    ghost function ToEqsAll(st: State): iset<State>
+    {
+        iset st' |
+          && |st'| == |st|
+          && forall i: Idx :: i < |st| && !(i in Prefix(0)) ==> st[i] == st'[i]
+    }
+
+    lemma PrefixLemma(n: nat)
+      requires n in Keys
+      requires n != 0
+      ensures Prefix(n) <= Remove0().Prefix(n)
+    {
+      if 0 in Keys {
+        forall i: Idx | i in Prefix(n) ensures i in Remove0().Prefix(n) {
+          var k :| k <= n && k in Keys && i in this[k];
+          if k != 0 {
+            assert k in Remove0().Keys;
+            assert this[k] <= Remove0()[k];
+          } else {
+            assert n in Remove0().Keys;
+          }
+        }
+      } else {
+        forall i: Idx | i in Prefix(n) ensures i in Remove0().Prefix(n) {
+          var k :| k <= n && k in Keys && i in this[k];
+          assert Remove0().Keys == Keys;
+          assert k in Remove0().Keys;
+        }
+      }
+    }
+
+    // lemma Prefix0All()
+    //   requires 0 in Keys
+    //   ensures Prefix(0) == AllVars()
+    // {
+    //   assert AllVars() <= Prefix(0);
+    //   assert Prefix(0) <= AllVars() by {
+    //     forall i: Idx | i in Prefix(0) ensures i in AllVars() {
+
+    //     }
+    //   }
+    // }
+  }
+
+  function Pred(n: nat): nat {
+    if n == 0 then 0 else n - 1
+  }
   
-//   function Process'(stmt: Stmt): VarsJumps 
-//     ensures forall v <- Process'(stmt).Values, s <- v :: s < stmt.Depth()
-//     decreases stmt
-//   {
-//     match stmt
-//     case Seq(ss) => SeqProcess'(ss)
-//     case Choice(s0, s1) => 
-//       var vs0 := Process'(s0);
-//       var vs1 := Process'(s1);
-//       vs0.Merge(vs1)
-//     case NewScope(n, s) => 
-//       var vs := Process'(s);
-//       vs.Substract(n)
-//     case Escape(n) => map[n := {}, 0 := {}]
-//     case Loop(inv, body) => Process'(body)[0 := {}]
-//     case Assign(x, _) => map[0 := {x}]
-//     case _ => map[0 := {}]
-//   }
+  function Process'(stmt: Stmt): VarsJumps 
+    ensures forall v <- Process'(stmt).Values, s <- v :: s < stmt.Depth()
+    decreases stmt
+  {
+    match stmt
+    case Seq(ss) => SeqProcess'(ss)
+    case Choice(s0, s1) => 
+      var vs0 := Process'(s0);
+      var vs1 := Process'(s1);
+      vs0.Merge(vs1)
+    case NewScope(n, s) => 
+      var vs := Process'(s);
+      vs.Substract(n)
+    case Escape(n) => map[n := {}]
+    /**
+      Loop
+        (x++) + (y++; exit 1)
+    We need to add all m[0] vars to other m[i] because 
+    loop modify 0 vars in first few operations and then
+    exit modify other vars
+    */
+    case Loop(inv, body) => Process'(body).Remove0()
+    case Assign(x, _) => map[0 := {x}]
+    case _ => map[0 := {}]
+  }
 
-//   function SeqProcess'(ss: seq<Stmt>): VarsJumps 
-//     ensures forall v <- SeqProcess'(ss).Values, s <- v :: s < SeqDepth(ss)
-//     decreases ss
-//   {
-//     if ss == [] then map[] else
-//       var v0 := Process'(ss[0]);
-//       if 0 in v0.Keys then
-//         v0.SeqMerge(SeqProcess'(ss[1..]))
-//       else v0
-//   }
-
-//   lemma Process'CorrectAux(stmt: Stmt, m: VarsJumps) 
-//     requires Process'(stmt) == m
-//     ensures forall v <- m.Values, s <- v :: s < stmt.Depth()
-//     ensures 0 in m.Keys
-//     ensures forall k <- m.Keys :: m[0] <= m[k]
-//   {
-//     match stmt 
-//     case Choice(s0, s1) =>
-//       var m0 := Process'(s0);
-//       var m1 := Process'(s1);
-//       Process'CorrectAux(s0, m0);
-//       Process'CorrectAux(s1, m1);
-//     case Loop(_, body) => 
-//     case NewScope(n, s) => 
-//       var m' := Process'(s);
-//       Process'CorrectAux(s, m');
-//     case Seq(ss) => SeqProcess'CorrectAux(ss, m);
-//     case _ => 
-//   }
-
-//   lemma SeqProcess'CorrectAux(ss: seq<Stmt>, m: VarsJumps) 
-//     requires SeqProcess'(ss) == m
-//     ensures forall v <- m.Values, s <- v :: s < SeqDepth(ss)
-//     ensures 0 in m.Keys
-//     ensures forall k <- m.Keys :: m[0] <= m[k]
-//   {
-
-//   }
-
-//   lemma Process'Correct(stmt: Stmt, st: State, m: VarsJumps, posts: Omni.Continuation) 
-//     requires Process'(stmt) == m
-//     ensures forall v <- m.Values, s <- v :: s < stmt.Depth()
-//     requires Omni.Sem(stmt, st, posts)
-//     ensures Omni.Sem(stmt, st, m.ToEqs(st, posts))
-//   {
-//     match stmt 
-//     case Choice(s0, s1) => 
-//       var m0 := Process'(s0);
-//       var m1 := Process'(s1);
-//       Omni.SemCons(s0, st, m0.ToEqs(st, posts), m0.Merge(m1).ToEqs(st, posts)) by {
-//         Process'Correct(s0, st, m0, posts);
-//       }
-//       Omni.SemCons(s1, st, m1.ToEqs(st, posts), m0.Merge(m1).ToEqs(st, posts)) by {
-//         Process'Correct(s1, st, m1, posts);
-//       }
-//     case Loop(_, body) =>  
-//       var inv :| 
-//         && st in inv
-//         && Omni.PreservesInv(inv, body, posts);
-//       var m' := Process'(body);
-//       var stvar := set i: Idx | i < |st|;
-//       Process'CorrectAux(body, m');
-//       var inv' := inv * m'.ToEqs(st, posts.UpdateHead(inv)).head;
-//       assert st in inv';
-//       forall st': State | st' in inv' ensures Omni.Sem(body, st', (m'[0 := {}]).ToEqs(st, posts).UpdateHead(inv')) {
-//         Omni.SemCons(body, st', m'.ToEqs(st', posts.UpdateHead(inv)), (m'[0 := {}]).ToEqs(st, posts).UpdateHead(inv')) by {
-//           Process'Correct(body, st', m', posts.UpdateHead(inv)) by {
-//             assert Omni.PreservesInv(inv, body, posts);
-//           }
-//         }
-//       }
-//     case NewScope(n, s) => assume false;
-//     case Seq(ss) => SeqProcess'Correct(ss, st, m, posts);
-//     case _ =>
-//   }
-
-//   lemma SeqProcess'Correct(ss: seq<Stmt>, st: State, m: VarsJumps, posts: Omni.Continuation) 
-//     requires SeqProcess'(ss) == m
-//     ensures forall v <- m.Values, s <- v :: s < SeqDepth(ss)
-//     requires Omni.SeqSem(ss, st, posts)
-//     ensures Omni.SeqSem(ss, st, m.ToEqs(st, posts))
-// /**
-//   ghost function AllStatesN(n: nat): Omni.Continuation 
-//     requires n > 0
-//   {
-//     seq(n, i => AllStates)
-//   }
-
-//   lemma Process'Correct(stmt: Stmt, st: State, m: VarsJumps, n: nat, posts: Omni.Continuation) 
-//     requires Process'(stmt) == (m, n)
-//     ensures forall v <- m.Keys :: v < stmt.Depth()
-//     requires Omni.Sem(stmt, st, posts)
-//     ensures Omni.Sem(stmt, st, m.ToEqs(st, n, posts))
-//   {
-//     match stmt
-//     case Choice(s0, s1) => 
-//       var (m0, n0) := Process'(s0);
-//       var (m1, n1) := Process'(s1);
-//       Omni.SemCons(s0, st, m0.ToEqs(st, n0, posts), m0.Merge(m1).ToEqs(st, min(n0, n1), posts)) by {
-//         assert m0.ToEqs(st, n0, posts).Leq(m0.Merge(m1).ToEqs(st, min(n0, n1), posts));
-//         Process'Correct(s0, st, m0, n0, posts);
-//       }
-//       Omni.SemCons(s1, st, m1.ToEqs(st, n1, posts), m0.Merge(m1).ToEqs(st, min(n0, n1), posts)) by {
-//         assert m1.ToEqs(st, n1, posts).Leq(m0.Merge(m1).ToEqs(st, min(n0, n1), posts));
-//         Process'Correct(s1, st, m1, n1, posts);
-//       }
-//     case Loop(_, body) => 
-//       var inv :| 
-//         && st in inv
-//         && Omni.PreservesInv(inv, body, posts);
-//       var inv' := inv * m.ToEqs(st, 0, posts.UpdateHead(inv)).head;
-//       assert st in inv';
-//       forall st': State | st' in inv' ensures Omni.Sem(body, st', m.ToEqs(st, n, posts).UpdateHead(inv')) {
-//         Omni.SemCons(body, st', m.ToEqs(st, n, posts.UpdateHead(inv')), m.ToEqs(st, n, posts).UpdateHead(inv')) by {
-//           assert Omni.Sem(body, st', m.ToEqs(st', n, posts.UpdateHead(inv'))) by {
-//             Omni.SemCons(body, st', m.ToEqs(st', n, posts.UpdateHead(inv)), m.ToEqs(st', n, posts.UpdateHead(inv'))) by {
-//               Process'Correct(body, st', m, n, posts.UpdateHead(inv)) by {
-//                 assert Omni.PreservesInv(inv, body, posts);
-//               }
-//               assert m.ToEqs(st', n, posts.UpdateHead(inv)).Leq(m.ToEqs(st', n, posts.UpdateHead(inv')));
-//             }
-//           }
-//           Omni.SemCons(body, st', m.ToEqs(st', n, posts.UpdateHead(inv')), m.ToEqs(st, n, posts.UpdateHead(inv')));
-//         }
-//       }
-//     case NewScope(k, body) =>
-//       forall vs: State | |vs| == k ensures Omni.Sem(body, st.Update(vs), m.ToEqs(st, n, posts).UpdateAndAdd(k)) {
-//         var (m', n') := Process'(body);
-//         Omni.SemCons(body, st.Update(vs), m'.ToEqs(st.Update(vs), n', posts.UpdateAndAdd(k)), m.ToEqs(st, n, posts).UpdateAndAdd(k)) by {
-//           Process'Correct(body, st.Update(vs), m', n', posts.UpdateAndAdd(k));
-//           assert m'.ToEqs(st.Update(vs), n', posts.UpdateAndAdd(k)).Leq(m'.Substract(k).ToEqs(st, Pred(n'), posts).UpdateAndAdd(k)) by {
-//             forall i: Idx | i < |posts| + 1 
-//               ensures m'.ToEqs(st.Update(vs), n', posts.UpdateAndAdd(k))[i] <=
-//                     m'.Substract(k).ToEqs(st, Pred(n'), posts).UpdateAndAdd(k)[i]
-//             {
-//               if i >= n' {
-//                 forall st': State | 
-//                   && st' in posts.UpdateAndAdd(k)[i]
-//                   && |st'| == |st| + k
-//                   && forall j: Idx :: j < |st| + k && !(j in m'.Keys && m'[j] <= i) ==> st.Update(vs)[j] == st'[j]
-//                   ensures
-//                     st' in m'.Substract(k).ToEqs(st, Pred(n'), posts).UpdateAndAdd(k)[i]
-//                 {
-//                   if i == 0 {
-//                     assert st'[k..] in m'.Substract(k).ToEqs(st, 0, posts).head by {
-//                       assert st'[k..] in posts.head by {
-//                         assert st' in posts.UpdateAndAdd(k)[0];
-//                         assert posts.UpdateAndAdd(k)[0] == UpdateSet(k, posts.head);
-//                       }
-//                       forall j: Idx | j < |st| && !(j in m'.Substract(k).Keys && m'.Substract(k)[j] <= 0) 
-//                         ensures st[j] == st'[j + k]
-//                       {
-//                         if j + k in m'.Keys && m'[j + k] <= 0 {
-//                           MaxLemma(m'.Keys, j, k);
-//                           assert j in m'.Substract(k).Keys && m'.Substract(k)[j] <= 0;
-//                         }
-//                         assert !(j + k in m'.Keys && m'[j + k] <= 0);
-//                       }
-//                     }
-//                   } else {
-//                     assert st'[k..] in m'.Substract(k).ToEqs(st, 0, posts)[i - 1] by {
-//                       assert st'[k..] in posts[i - 1] by {
-//                         assert st' in posts.UpdateAndAdd(k)[i];
-//                         assert posts.UpdateAndAdd(k)[i] == UpdateSet(k, posts[i - 1]);
-//                       }
-//                       forall j: Idx | j < |st| && !(j in m'.Substract(k).Keys && m'.Substract(k)[j] <= i - 1) 
-//                         ensures st[j] == st'[j + k]
-//                       {
-//                         if j + k in m'.Keys && m'[j + k] <= i {
-//                           MaxLemma(m'.Keys, j, k);
-//                           assert j in m'.Substract(k).Keys && m'.Substract(k)[j] <= i - 1;
-//                         }
-//                         assert !(j + k in m'.Keys && m'[j + k] <= i);
-//                       }
-//                     }
-//                   }
-//                 }
-//               }
-//             }
-//           }
-//         }
-//       }
-//     case Seq(ss) => SeqProcess'Correct(ss, st, m, n, posts);
-//     case _ =>
-//   }
-
-//   lemma SeqProcess'Correct(ss: seq<Stmt>, st: State, m: VarsJumps, n: nat, posts: Omni.Continuation) 
-//     requires SeqProcess'(ss) == (m, n)
-//     ensures forall v <- m.Keys :: v < SeqDepth(ss)
-//     requires Omni.SeqSem(ss, st, posts)
-//     ensures Omni.SeqSem(ss, st, m.ToEqs(st, n, posts))
-//   {
-//     if ss != [] {
-//       Omni.SemNest(ss[0], ss[1..], st, m.ToEqs(st, n, posts)) by {
-//         assert Omni.Sem(ss[0], st, m.ToEqs(st, n, posts).UpdateHead(Omni.SeqWP(ss[1..],  m.ToEqs(st, n, posts)))) by {
-//           assert Omni.Sem(ss[0], st, posts.UpdateHead(Omni.SeqWP(ss[1..], posts)));
-//           var (m', n') := Process'(ss[0]);
-//           Process'Correct(ss[0], st, m', n', posts.UpdateHead(Omni.SeqWP(ss[1..], posts)));
-//           assert Omni.Sem(ss[0], st, m'.ToEqs(st, n', posts.UpdateHead(Omni.SeqWP(ss[1..], posts))));
-//           if n' != 0 {
-//             Omni.SemCons(ss[0], st, m'.ToEqs(st, n', posts.UpdateHead(Omni.SeqWP(ss[1..], posts))), 
-//               m.ToEqs(st, n, posts).UpdateHead(Omni.SeqWP(ss[1..], m.ToEqs(st, n, posts))));
-//           } else {
-//             var (m'', n'') := SeqProcess'(ss[1..]);
-//             assert m == m'.Update(n'').Merge(m'');
-//             assert n == n'';
-//             // ???
-//             // forall st' | Omni.SeqSem(ss[1..], st', posts) { SeqProcess'Correct(ss[1..], st', m'', n'', posts); }
-//             Omni.SemCons(ss[0], st, m'.ToEqs(st, n', posts.UpdateHead(Omni.SeqWP(ss[1..], posts))), 
-//               m.ToEqs(st, n, posts).UpdateHead(Omni.SeqWP(ss[1..], m.ToEqs(st, n, posts)))) by 
-//             {
-//               forall i: Idx | i < |posts| 
-//                 ensures m'.ToEqs(st, n', posts.UpdateHead(Omni.SeqWP(ss[1..], posts)))[i] <= 
-//                       m.ToEqs(st, n, posts).UpdateHead(Omni.SeqWP(ss[1..], m.ToEqs(st, n, posts)))[i] 
-//               {
-//                 if i >= n' {
-//                   forall st': State | st' in m'.ToEqs(st, n', posts.UpdateHead(Omni.SeqWP(ss[1..], posts)))[i] 
-//                     ensures st' in m.ToEqs(st, n, posts).UpdateHead(Omni.SeqWP(ss[1..], m.ToEqs(st, n, posts)))[i] 
-//                   {
-//                     if i == 0 {
-//                       assert Omni.SeqSem(ss[1..], st', posts);
-//                       SeqProcess'Correct(ss[1..], st', m'', n'', posts);
-//                       Omni.SeqSemCons(ss[1..], st', m''.ToEqs(st', n'', posts), m.ToEqs(st, n, posts));
-//                       assert Omni.SeqSem(ss[1..], st', m.ToEqs(st, n, posts));
-//                     } else {
-//                       assert |st'| == |st|;
-//                       assert st' in posts[i];
-//                       assert forall j: Idx :: j < |st| && !(j in m'.Keys && m'[j] <= i) ==> st[j] == st'[j];
-//                       assert st' in m.ToEqs(st, n, posts)[i] by {
-//                         assert n' == 0;
-//                         assert n == n'';
-//                         forall j: Idx | j < |st| && !(j in m.Keys && m[j] <= i) 
-//                           ensures st[j] == st'[j]
-//                         {
-//                           assume false;
-//                         }
-//                       }
-//                     }
-//                   }
-//                 }
-//               }
-//             }
-//           }
-//         }
-//       }
-//     }
-//   }*/
-
-//   function Process(stmt: Stmt): set<Idx> 
-//     ensures forall v <- Process(stmt) :: v < stmt.Depth()
-//   {
-//     {}
-//     // var (vs, n) := Process'(stmt);
-//     // if n == 0 then set i | i in vs.Keys && vs[i] == 0 else {}
-//   } 
+  function SeqProcess'(ss: seq<Stmt>): VarsJumps 
+    ensures forall v <- SeqProcess'(ss).Values, s <- v :: s < SeqDepth(ss)
+    decreases ss
+  {
+    if ss == [] then map[] else
+      var v0 := Process'(ss[0]);
+      if 0 in v0.Keys then
+        v0.SeqMerge(SeqProcess'(ss[1..]))
+      else v0
+  }
 
 
+  // verification-time-limit 40
+  lemma Process'Correct(stmt: Stmt, st: State, m: VarsJumps, posts: Omni.Continuation) 
+    requires Process'(stmt) == m
+    ensures forall v <- m.Values, s <- v :: s < stmt.Depth()
+    requires Omni.Sem(stmt, st, posts)
+    ensures Omni.Sem(stmt, st, m.ToEqs(st, posts))
+  {
+    match stmt 
+    case Choice(s0, s1) => assume false;
+      // var m0 := Process'(s0);
+      // var m1 := Process'(s1);
+      // Omni.SemCons(s0, st, m0.ToEqs(st, posts), m0.Merge(m1).ToEqs(st, posts)) by {
+      //   Process'Correct(s0, st, m0, posts);
+      // }
+      // Omni.SemCons(s1, st, m1.ToEqs(st, posts), m0.Merge(m1).ToEqs(st, posts)) by {
+      //   Process'Correct(s1, st, m1, posts);
+      // }
+    case Loop(_, body) =>  assume false;
+      // var inv :| 
+      //   && st in inv
+      //   && Omni.PreservesInv(inv, body, posts);
+      // var m' := Process'(body);
+      // var inv' := inv * m'.ToEqsAll(st);
+      // assert st in inv';
+      // forall st': State | st' in inv' ensures Omni.Sem(body, st', (m'.Remove0()).ToEqs(st, posts).UpdateHead(inv')) {
+      //   Omni.SemCons(body, st', m'.ToEqs(st', posts.UpdateHead(inv)), (m'.Remove0()).ToEqs(st, posts).UpdateHead(inv')) by {
+      //     assert m'.ToEqs(st', posts.UpdateHead(inv)).Leq((m'.Remove0()).ToEqs(st, posts).UpdateHead(inv')) by {
+      //       forall i: Idx | i < |posts| 
+      //         ensures m'.ToEqs(st', posts.UpdateHead(inv))[i] <= (m'.Remove0()).ToEqs(st, posts).UpdateHead(inv')[i]
+      //       {
+      //         forall st'': State | st'' in m'.ToEqs(st', posts.UpdateHead(inv))[i]
+      //           ensures st'' in (m'.Remove0()).ToEqs(st, posts).UpdateHead(inv')[i]
+      //         {
+      //           if i in m'.Keys  {
+      //             if i == 0 {
+      //               if 0 in m'.Keys {
+      //                 assert st'' in inv;
+      //               }
+      //             } else {
+      //               assert forall j: Idx :: j < |st'| && !(j in m'.Prefix(i)) ==> st'[j] == st''[j];
+      //               assert forall j: Idx :: j < |st| && !(j in m'.Prefix(0)) ==> st[j] == st'[j];
+      //               forall j: Idx | j < |st| && !(j in (m'.Remove0()).Prefix(i))
+      //                 ensures st[j] == st''[j]
+      //               {
+      //                 m'.PrefixLemma(i);
+      //                 assert m'.Prefix(0) <= m'.Remove0().Prefix(i);
+      //               }
+      //             }
+      //           }
+      //         }
+      //       }
+      //     }
+      //     Process'Correct(body, st', m', posts.UpdateHead(inv)) by {
+      //       assert Omni.PreservesInv(inv, body, posts);
+      //     }
+      //   }
+      // }
+    case NewScope(n, s) => 
+      forall vs: State | |vs| == n ensures Omni.Sem(s, st.Update(vs), m.ToEqs(st, posts).UpdateAndAdd(n)) {
+        var m' := Process'(s);
+        Omni.SemCons(s, st.Update(vs), m'.ToEqs(st.Update(vs), posts.UpdateAndAdd(n)), m.ToEqs(st, posts).UpdateAndAdd(n)) by {
+          Process'Correct(s, st.Update(vs), m', posts.UpdateAndAdd(n));
+          forall i: Idx | i < |posts| + 1 
+            ensures m'.ToEqs(st.Update(vs), posts.UpdateAndAdd(n))[i] <=
+              m'.Substract(n).ToEqs(st, posts).UpdateAndAdd(n)[i]
+          {
+            forall st': State | st' in m'.ToEqs(st.Update(vs), posts.UpdateAndAdd(n))[i] 
+              ensures st' in m'.Substract(n).ToEqs(st, posts).UpdateAndAdd(n)[i]
+            {
+              assert |st'| == |st| + n;
+              assert st' in posts.UpdateAndAdd(n)[i];
+              if i == 0 {
+                assert st'[n..] in m'.Substract(n).ToEqs(st, posts).head by {
+                  // assume false;
+                  if 0 in m'.Keys {
+                    assert Pred(0) in m'.Keys;
+                    assert 0 in m'.Substract(n).Keys;
+                  }
+                }
+              } else {
+                assert st'[n..] in m'.Substract(n).ToEqs(st, posts)[i - 1] by {
+                  if i in m'.Keys {
+                  // assume false;
+                    assert |st| + n == |st'|;
+                    assert st'[n..] in posts[i -1] by {
+                      assert i > 0;
+                      assert st' in posts.UpdateAndAdd(n)[i];
+                      assert ([posts.head] + posts)[i] == posts[i - 1];
+                      assert st' in UpdateSet(n, posts[i - 1]);
+                    }
+                    assert forall j: Idx :: j < |st| + n && !(j in m'.Prefix(i)) ==> st.Update(vs)[j] == st'[j];
+                    assert i - 1 <= Max'(m'.Keys) + 1;
+                    assert (i - 1) in m'.Substract(n).Keys;
+                    assert m'.Prefix(i) <= m'.Substract(n).Prefix(i - 1) by {
+                      assume false;
+                    }
+                    assume false;
+                    // assume false;
+                    // if i == 1 {
+                    //   assert (i - 1) in m'.Substract(n).Keys;
+                    // } else {
+                    //   assume false;
+                    // }
+                  }
+                }
+              }
+            }
+          }
+        }
+      }
+    case Seq(ss) => SeqProcess'Correct(ss, st, m, posts);
+    case _ =>
+  }
 
-//   // function Process(stmt: Stmt): (set<Idx>, bool) 
-//   //   ensures forall v <- Process(stmt).0 :: v < stmt.Depth()
-//   //   decreases stmt
-//   // {
-//   //   match stmt
-//   //   case Seq(ss) => SeqProcess(ss)
-//   //   case Choice(s0, s1) => 
-//   //     var (vs0, b0) := Process(s0);
-//   //     var (vs1, b1) := Process(s1);
-//   //     (vs0 + vs1, b0 || b1)
-//   //   case NewScope(n, s) => 
-//   //     var (vs, b) := Process(s);
-//   //     (Substract(vs, n), b)
-//   //   case Escape(_) => ({}, false)
-//   //   case Loop(inv, body) => Process(body)
-//   //   case Assign(x, _) => ({x}, true)
-//   //   case _ => ({}, true)
-//   // }
+  lemma SeqProcess'Correct(ss: seq<Stmt>, st: State, m: VarsJumps, posts: Omni.Continuation) 
+    requires SeqProcess'(ss) == m
+    ensures forall v <- m.Values, s <- v :: s < SeqDepth(ss)
+    requires Omni.SeqSem(ss, st, posts)
+    ensures Omni.SeqSem(ss, st, m.ToEqs(st, posts))
+/**
+  ghost function AllStatesN(n: nat): Omni.Continuation 
+    requires n > 0
+  {
+    seq(n, i => AllStates)
+  }
 
-//   // function SeqProcess(ss: seq<Stmt>): (set<Idx>, bool) 
-//   //   ensures forall v <- SeqProcess(ss).0 :: v < SeqDepth(ss)
-//   //   decreases ss
-//   // {
-//   //   if ss == [] then ({}, true) else
-//   //     var (v0, b0) := Process(ss[0]);
-//   //     if b0 then
-//   //       var (v1, b1) := SeqProcess(ss[1..]);
-//   //       (v0 + v1, b0 || b1)
-//   //     else
-//   //       (v0, b0)
-//   // }
+  lemma Process'Correct(stmt: Stmt, st: State, m: VarsJumps, n: nat, posts: Omni.Continuation) 
+    requires Process'(stmt) == (m, n)
+    ensures forall v <- m.Keys :: v < stmt.Depth()
+    requires Omni.Sem(stmt, st, posts)
+    ensures Omni.Sem(stmt, st, m.ToEqs(st, n, posts))
+  {
+    match stmt
+    case Choice(s0, s1) => 
+      var (m0, n0) := Process'(s0);
+      var (m1, n1) := Process'(s1);
+      Omni.SemCons(s0, st, m0.ToEqs(st, n0, posts), m0.Merge(m1).ToEqs(st, min(n0, n1), posts)) by {
+        assert m0.ToEqs(st, n0, posts).Leq(m0.Merge(m1).ToEqs(st, min(n0, n1), posts));
+        Process'Correct(s0, st, m0, n0, posts);
+      }
+      Omni.SemCons(s1, st, m1.ToEqs(st, n1, posts), m0.Merge(m1).ToEqs(st, min(n0, n1), posts)) by {
+        assert m1.ToEqs(st, n1, posts).Leq(m0.Merge(m1).ToEqs(st, min(n0, n1), posts));
+        Process'Correct(s1, st, m1, n1, posts);
+      }
+    case Loop(_, body) => 
+      var inv :| 
+        && st in inv
+        && Omni.PreservesInv(inv, body, posts);
+      var inv' := inv * m.ToEqs(st, 0, posts.UpdateHead(inv)).head;
+      assert st in inv';
+      forall st': State | st' in inv' ensures Omni.Sem(body, st', m.ToEqs(st, n, posts).UpdateHead(inv')) {
+        Omni.SemCons(body, st', m.ToEqs(st, n, posts.UpdateHead(inv')), m.ToEqs(st, n, posts).UpdateHead(inv')) by {
+          assert Omni.Sem(body, st', m.ToEqs(st', n, posts.UpdateHead(inv'))) by {
+            Omni.SemCons(body, st', m.ToEqs(st', n, posts.UpdateHead(inv)), m.ToEqs(st', n, posts.UpdateHead(inv'))) by {
+              Process'Correct(body, st', m, n, posts.UpdateHead(inv)) by {
+                assert Omni.PreservesInv(inv, body, posts);
+              }
+              assert m.ToEqs(st', n, posts.UpdateHead(inv)).Leq(m.ToEqs(st', n, posts.UpdateHead(inv')));
+            }
+          }
+          Omni.SemCons(body, st', m.ToEqs(st', n, posts.UpdateHead(inv')), m.ToEqs(st, n, posts.UpdateHead(inv')));
+        }
+      }
+    case NewScope(k, body) =>
+      forall vs: State | |vs| == k ensures Omni.Sem(body, st.Update(vs), m.ToEqs(st, n, posts).UpdateAndAdd(k)) {
+        var (m', n') := Process'(body);
+        Omni.SemCons(body, st.Update(vs), m'.ToEqs(st.Update(vs), n', posts.UpdateAndAdd(k)), m.ToEqs(st, n, posts).UpdateAndAdd(k)) by {
+          Process'Correct(body, st.Update(vs), m', n', posts.UpdateAndAdd(k));
+          assert m'.ToEqs(st.Update(vs), n', posts.UpdateAndAdd(k)).Leq(m'.Substract(k).ToEqs(st, Pred(n'), posts).UpdateAndAdd(k)) by {
+            forall i: Idx | i < |posts| + 1 
+              ensures m'.ToEqs(st.Update(vs), n', posts.UpdateAndAdd(k))[i] <=
+                    m'.Substract(k).ToEqs(st, Pred(n'), posts).UpdateAndAdd(k)[i]
+            {
+              if i >= n' {
+                forall st': State | 
+                  && st' in posts.UpdateAndAdd(k)[i]
+                  && |st'| == |st| + k
+                  && forall j: Idx :: j < |st| + k && !(j in m'.Keys && m'[j] <= i) ==> st.Update(vs)[j] == st'[j]
+                  ensures
+                    st' in m'.Substract(k).ToEqs(st, Pred(n'), posts).UpdateAndAdd(k)[i]
+                {
+                  if i == 0 {
+                    assert st'[k..] in m'.Substract(k).ToEqs(st, 0, posts).head by {
+                      assert st'[k..] in posts.head by {
+                        assert st' in posts.UpdateAndAdd(k)[0];
+                        assert posts.UpdateAndAdd(k)[0] == UpdateSet(k, posts.head);
+                      }
+                      forall j: Idx | j < |st| && !(j in m'.Substract(k).Keys && m'.Substract(k)[j] <= 0) 
+                        ensures st[j] == st'[j + k]
+                      {
+                        if j + k in m'.Keys && m'[j + k] <= 0 {
+                          MaxLemma(m'.Keys, j, k);
+                          assert j in m'.Substract(k).Keys && m'.Substract(k)[j] <= 0;
+                        }
+                        assert !(j + k in m'.Keys && m'[j + k] <= 0);
+                      }
+                    }
+                  } else {
+                    assert st'[k..] in m'.Substract(k).ToEqs(st, 0, posts)[i - 1] by {
+                      assert st'[k..] in posts[i - 1] by {
+                        assert st' in posts.UpdateAndAdd(k)[i];
+                        assert posts.UpdateAndAdd(k)[i] == UpdateSet(k, posts[i - 1]);
+                      }
+                      forall j: Idx | j < |st| && !(j in m'.Substract(k).Keys && m'.Substract(k)[j] <= i - 1) 
+                        ensures st[j] == st'[j + k]
+                      {
+                        if j + k in m'.Keys && m'[j + k] <= i {
+                          MaxLemma(m'.Keys, j, k);
+                          assert j in m'.Substract(k).Keys && m'.Substract(k)[j] <= i - 1;
+                        }
+                        assert !(j + k in m'.Keys && m'[j + k] <= i);
+                      }
+                    }
+                  }
+                }
+              }
+            }
+          }
+        }
+      }
+    case Seq(ss) => SeqProcess'Correct(ss, st, m, n, posts);
+    case _ =>
+  }
 
-//   function PairToSet(p: (set<Idx>, bool)): set<Idx> {
-//     if p.1 then p.0 else {}
-//   }
+  lemma SeqProcess'Correct(ss: seq<Stmt>, st: State, m: VarsJumps, n: nat, posts: Omni.Continuation) 
+    requires SeqProcess'(ss) == (m, n)
+    ensures forall v <- m.Keys :: v < SeqDepth(ss)
+    requires Omni.SeqSem(ss, st, posts)
+    ensures Omni.SeqSem(ss, st, m.ToEqs(st, n, posts))
+  {
+    if ss != [] {
+      Omni.SemNest(ss[0], ss[1..], st, m.ToEqs(st, n, posts)) by {
+        assert Omni.Sem(ss[0], st, m.ToEqs(st, n, posts).UpdateHead(Omni.SeqWP(ss[1..],  m.ToEqs(st, n, posts)))) by {
+          assert Omni.Sem(ss[0], st, posts.UpdateHead(Omni.SeqWP(ss[1..], posts)));
+          var (m', n') := Process'(ss[0]);
+          Process'Correct(ss[0], st, m', n', posts.UpdateHead(Omni.SeqWP(ss[1..], posts)));
+          assert Omni.Sem(ss[0], st, m'.ToEqs(st, n', posts.UpdateHead(Omni.SeqWP(ss[1..], posts))));
+          if n' != 0 {
+            Omni.SemCons(ss[0], st, m'.ToEqs(st, n', posts.UpdateHead(Omni.SeqWP(ss[1..], posts))), 
+              m.ToEqs(st, n, posts).UpdateHead(Omni.SeqWP(ss[1..], m.ToEqs(st, n, posts))));
+          } else {
+            var (m'', n'') := SeqProcess'(ss[1..]);
+            assert m == m'.Update(n'').Merge(m'');
+            assert n == n'';
+            // ???
+            // forall st' | Omni.SeqSem(ss[1..], st', posts) { SeqProcess'Correct(ss[1..], st', m'', n'', posts); }
+            Omni.SemCons(ss[0], st, m'.ToEqs(st, n', posts.UpdateHead(Omni.SeqWP(ss[1..], posts))), 
+              m.ToEqs(st, n, posts).UpdateHead(Omni.SeqWP(ss[1..], m.ToEqs(st, n, posts)))) by 
+            {
+              forall i: Idx | i < |posts| 
+                ensures m'.ToEqs(st, n', posts.UpdateHead(Omni.SeqWP(ss[1..], posts)))[i] <= 
+                      m.ToEqs(st, n, posts).UpdateHead(Omni.SeqWP(ss[1..], m.ToEqs(st, n, posts)))[i] 
+              {
+                if i >= n' {
+                  forall st': State | st' in m'.ToEqs(st, n', posts.UpdateHead(Omni.SeqWP(ss[1..], posts)))[i] 
+                    ensures st' in m.ToEqs(st, n, posts).UpdateHead(Omni.SeqWP(ss[1..], m.ToEqs(st, n, posts)))[i] 
+                  {
+                    if i == 0 {
+                      assert Omni.SeqSem(ss[1..], st', posts);
+                      SeqProcess'Correct(ss[1..], st', m'', n'', posts);
+                      Omni.SeqSemCons(ss[1..], st', m''.ToEqs(st', n'', posts), m.ToEqs(st, n, posts));
+                      assert Omni.SeqSem(ss[1..], st', m.ToEqs(st, n, posts));
+                    } else {
+                      assert |st'| == |st|;
+                      assert st' in posts[i];
+                      assert forall j: Idx :: j < |st| && !(j in m'.Keys && m'[j] <= i) ==> st[j] == st'[j];
+                      assert st' in m.ToEqs(st, n, posts)[i] by {
+                        assert n' == 0;
+                        assert n == n'';
+                        forall j: Idx | j < |st| && !(j in m.Keys && m[j] <= i) 
+                          ensures st[j] == st'[j]
+                        {
+                          assume false;
+                        }
+                      }
+                    }
+                  }
+                }
+              }
+            }
+          }
+        }
+      }
+    }
+  }*/
 
-//   ghost function EqsTo(vars: set<Idx>, st: State): iset<State> 
-//     requires forall v <- vars :: v < |st|
-//   {
-//     iset st': State | 
-//       && |st'| == |st|
-//       && forall i: Idx :: i < |st| && i !in vars ==> st'[i] == st[i]
-//   }
+  function Process(stmt: Stmt): set<Idx> 
+    ensures forall v <- Process(stmt) :: v < stmt.Depth()
+  {
+    {}
+    // var (vs, n) := Process'(stmt);
+    // if n == 0 then set i | i in vs.Keys && vs[i] == 0 else {}
+  } 
 
 
-//   lemma Correct'(stmt: Stmt, st: State, vars: set<Idx>, posts: Omni.Continuation, b : bool) 
-//     requires forall v <- vars :: v < |st|
-//     requires Omni.Sem(stmt, st, posts)
-//     requires Process(stmt) == vars
-//     ensures Omni.Sem(stmt, st, posts.UpdateHead(posts.head * EqsTo(vars, st)))
 
-//   lemma Correct(stmt: Stmt, st: State, st': State, vars: set<Idx>, posts: Omni.Continuation, post: iset<State>) 
-//     requires forall v <- vars :: v < |st'|
-//     requires Omni.Sem(stmt, st, posts.UpdateHead(post))
-//     requires Process(stmt) == vars
-//     requires st in EqsTo(vars, st')
-//     ensures Omni.Sem(stmt, st, posts.UpdateHead(post * EqsTo(vars, st')))
+  // function Process(stmt: Stmt): (set<Idx>, bool) 
+  //   ensures forall v <- Process(stmt).0 :: v < stmt.Depth()
+  //   decreases stmt
+  // {
+  //   match stmt
+  //   case Seq(ss) => SeqProcess(ss)
+  //   case Choice(s0, s1) => 
+  //     var (vs0, b0) := Process(s0);
+  //     var (vs1, b1) := Process(s1);
+  //     (vs0 + vs1, b0 || b1)
+  //   case NewScope(n, s) => 
+  //     var (vs, b) := Process(s);
+  //     (Substract(vs, n), b)
+  //   case Escape(_) => ({}, false)
+  //   case Loop(inv, body) => Process(body)
+  //   case Assign(x, _) => ({x}, true)
+  //   case _ => ({}, true)
+  // }
+
+  // function SeqProcess(ss: seq<Stmt>): (set<Idx>, bool) 
+  //   ensures forall v <- SeqProcess(ss).0 :: v < SeqDepth(ss)
+  //   decreases ss
+  // {
+  //   if ss == [] then ({}, true) else
+  //     var (v0, b0) := Process(ss[0]);
+  //     if b0 then
+  //       var (v1, b1) := SeqProcess(ss[1..]);
+  //       (v0 + v1, b0 || b1)
+  //     else
+  //       (v0, b0)
+  // }
+
+  function PairToSet(p: (set<Idx>, bool)): set<Idx> {
+    if p.1 then p.0 else {}
+  }
+
+  ghost function EqsTo(vars: set<Idx>, st: State): iset<State> 
+    requires forall v <- vars :: v < |st|
+  {
+    iset st': State | 
+      && |st'| == |st|
+      && forall i: Idx :: i < |st| && i !in vars ==> st'[i] == st[i]
+  }
+
+
+  lemma Correct'(stmt: Stmt, st: State, vars: set<Idx>, posts: Omni.Continuation, b : bool) 
+    requires forall v <- vars :: v < |st|
+    requires Omni.Sem(stmt, st, posts)
+    requires Process(stmt) == vars
+    ensures Omni.Sem(stmt, st, posts.UpdateHead(posts.head * EqsTo(vars, st)))
+
+  lemma Correct(stmt: Stmt, st: State, st': State, vars: set<Idx>, posts: Omni.Continuation, post: iset<State>) 
+    requires forall v <- vars :: v < |st'|
+    requires Omni.Sem(stmt, st, posts.UpdateHead(post))
+    requires Process(stmt) == vars
+    requires st in EqsTo(vars, st')
+    ensures Omni.Sem(stmt, st, posts.UpdateHead(post * EqsTo(vars, st')))
     
-// }
+}
